Filesys/PathBasedFSRefinement.i.dfy
@@ -1,0 +1,208 @@
+// Copyright 2018-2021 VMware, Inc., Microsoft Inc., Carnegie Mellon University, ETH Zurich, and University of Washington
+// SPDX-License-Identifier: BSD-2-Clause
+
+include "FileSystem.s.dfy"
+include "PathBasedFSInv.i.dfy"
+
+module PathBasedFSRefinement {
+  import F = FileSystem
+  import P = PathBasedFS
+  import PInv = PathBasedFSInv
+  import opened Options
+  import opened FSTypes
+  import opened PathSpec
+
+  /// Interpretation Functions
+
+  function IPathMap(fs: P.FileSys) : (F.PathMap)
+  requires PInv.Inv(fs)
+  {
+    imap path :: if P.PathExists(fs, path) then P.GetMeta(fs, path).id else Nonexistent
+  }
+
+  function IMetaMap(fs: P.FileSys) : (F.MetaView)
+  requires PInv.Inv(fs)
+  {
+    var path_map := IPathMap(fs);
+
+    imap id : ID :: 
+      if id in path_map.Values 
+      then var p :| p in path_map && path_map[p] == id; P.GetMeta(fs, p)
+      else EmptyMeta
+  }
+
+  function IDataMap(fs: P.FileSys) : (F.DataView)
+  requires PInv.Inv(fs)
+  {
+    var path_map := IPathMap(fs);
+
+    imap id : ID :: 
+      if id in path_map.Values
+      then var p :| p in path_map && path_map[p] == id; P.GetData(fs, p)
+      else EmptyData()
+  }
+
+  function IStep(step: P.Step) : (i_step: F.Step)
+  {
+    match step {
+      case GetAttrStep(path, attr) => F.GetAttrStep(path, attr)
+      case ReadLinkStep(path, link_path) => F.ReadLinkStep(path, link_path)
+      case CreateStep(path, m) => F.CreateStep(path, m)
+      case DeleteStep(path, ctime) => F.DeleteStep(path, ctime)
+      case RenameStep(source, dest, ctime) => F.RenameStep(source, dest, ctime)
+      case LinkStep(source, dest, ctime, hiddenName) => F.LinkStep(source, dest, ctime)
+      case ChangeAttrStep(path, perm, uid, gid, ctime) => F.ChangeAttrStep(path, perm, uid, gid, ctime)
+      case TruncateStep(path, size, time) => F.TruncateStep(path, size, time)
+      case ReadStep(path, offset, size, data) => F.ReadStep(path, offset, size, data)
+      case WriteStep(path, offset, size, data, time) => F.WriteStep(path, offset, size, data, time)
+      case UpdateTimeStep(path, atime, mtime, ctime) => F.UpdateTimeStep(path, atime, mtime, ctime)
+      case ReadDirStep(dir, start, results, done) => F.ReadDirStep(dir, start, results, done)
+      case _ => F.StutterStep
+    }
+  }
+
+  function I(fs: P.FileSys) : (F.FileSys)
+  requires PInv.Inv(fs)
+  {
+    F.FileSys(IPathMap(fs), IMetaMap(fs), IDataMap(fs))
+  }
+
+  /// Refinement Proofs
+
+  lemma PathExistsEquiv(fs: P.FileSys, path: Path)
+  requires PInv.Inv(fs)
+  requires P.PathExists(fs, path)
+  ensures F.PathExists(I(fs), path)
+  {
+  }
+
+  lemma GetMetaEquiv(fs: P.FileSys, path: Path)
+  requires PInv.Inv(fs)
+  ensures P.GetMeta(fs, path) == I(fs).meta_map[I(fs).path_map[path]]
+  {
+  }
+
+  lemma NoAliasEquiv(fs: P.FileSys, path: Path)
+  requires PInv.Inv(fs)
+  requires P.PathExists(fs, path)
+  ensures P.NoAlias(fs, path) == F.NoAlias(I(fs), path)
+  {
+  }
+
+  lemma RefinesInit(fs: P.FileSys)
+  requires P.Init(fs)
+  requires PInv.Inv(fs)
+  ensures F.Init(I(fs))
+  {
+    assert I(fs).path_map[RootDir] == RootID; // observe
+  }
+
+  lemma RefinesNext(fs: P.FileSys, fs': P.FileSys)
+  requires PInv.Inv(fs)
+  requires P.Next(fs, fs')
+  ensures PInv.Inv(fs')
+  ensures F.Next(I(fs), I(fs'))
+  {
+    var step :| P.NextStep(fs, fs', step);
+    NextStepPreservesInv(fs, fs', step);
+  }
+
+  lemma NextStepPreservesInv(fs: P.FileSys, fs': P.FileSys, step: P.Step)
+  requires PInv.Inv(fs)
+  requires P.NextStep(fs, fs', step)
+  ensures PInv.Inv(fs')
+  ensures F.NextStep(I(fs), I(fs'), IStep(step))
+  {
+    var i_step := IStep(step);
+
+    match step {
+      case GetAttrStep(path, ctime) => RefinesGetAttr(fs, fs', path, ctime);
+      case ReadLinkStep(path, link_path) => RefinesReadLink(fs, fs', path, link_path);
+      case CreateStep(path, m) => RefinesCreate(fs, fs', path, m);
+
+      // ===== TBD =====
+      case DeleteStep(path, ctime) => RefinesDelete(fs, fs', path, ctime);
+      case RenameStep(source, dest, ctime) => {
+        assert i_step == F.RenameStep(source, dest, ctime); // observe
+        RefinesRename(fs, fs', source, dest, ctime);
+      } 
+      case LinkStep(source, dest, ctime, hiddenName) => {
+        assert i_step == F.LinkStep(source, dest, ctime); // observe
+        RefinesLink(fs, fs', source, dest, ctime, hiddenName);
+      }
+      case _ => {
+        assume false;
+      }
+    }
+  }
+
+  lemma RefinesGetAttr(fs: P.FileSys, fs': P.FileSys, path: Path, attr: MetaData)
+  requires PInv.Inv(fs)
+  requires P.GetAttr(fs, fs', path, attr)
+  ensures F.GetAttr(I(fs), I(fs'), path, attr)
+  {
+  }
+
+  lemma RefinesReadLink(fs: P.FileSys, fs': P.FileSys, path: Path, link_path: Path)
+  requires PInv.Inv(fs)
+  requires P.ReadLink(fs, fs', path, link_path)
+  ensures F.ReadLink(I(fs), I(fs'), path, link_path)
+  {
+  }
+
+  lemma RefinesCreate(fs: P.FileSys, fs': P.FileSys, path: Path, m: MetaData)
+  requires PInv.Inv(fs)
+  requires P.Create(fs, fs', path, m)
+  ensures PInv.Inv(fs')
+  ensures F.Create(I(fs), I(fs'), path, m)
+  {
+
+    // how to refine create
+
+
+    // PathExistsEquiv(fs, path);
+    // GetMetaEquiv(fs, path);
+
+    assume false;
+  }
+
+  lemma RefinesDelete(fs: P.FileSys, fs': P.FileSys, path: Path, ctime: Time)
+  requires PInv.Inv(fs)
+  requires P.Delete(fs, fs', path, ctime)
+  ensures PInv.Inv(fs')
+  ensures F.Delete(I(fs), I(fs'), path, ctime)
+  {
+    assume false;
+  }
+
+  lemma RefinesRename(fs: P.FileSys, fs': P.FileSys, source: Path, dest: Path, ctime: Time)
+  requires PInv.Inv(fs)
+  requires P.Rename(fs, fs', source, dest, ctime)
+  ensures PInv.Inv(fs')
+  ensures F.Rename(I(fs), I(fs'), source, dest, ctime)
+  {
+    assume false;
+  }
+
+  lemma RefinesLink(fs: P.FileSys, fs': P.FileSys, source: Path, dest: Path, ctime: Time, hiddenName: Option<Path>)
+  requires PInv.Inv(fs)
+  requires P.Link(fs, fs', source, dest, ctime, hiddenName)
+  ensures PInv.Inv(fs')
+  ensures F.Link(I(fs), I(fs'), source, dest, ctime)
+  {
+    assume false;
+  }
+
+  // lemma RefinesSimpleStep(fs: P.FileSys, fs': P.FileSys, step: P.Step)
+  // requires PInv.Inv(fs)
+  // requires P.NextStep(fs, fs', step)
+  // requires step.CreateStep? || step.ChangeAttrStep? || step.TruncateStep? || step.WriteStep? || step.UpdateTimeStep?
+  // ensures PInv.Inv(fs')
+  // ensures F.NextStep(I(fs), I(fs'), IStep(step))
+  // {
+  //   assume false;
+  // }
+
+  // maybe for simple ones
+
+}
